\noindent
\begin{minipage}{0.4\linewidth}
    \parbox[t]{0.35\linewidth}
    {
        \begin{alignat*}{2}
            & z &&= \frac{u}{v} \\
            & &&= \frac{u}{v} \cdot \frac{\bar{v}}{\bar{v}} \\
            & &&= \frac{u \cdot \bar{v}}{v \cdot \bar{v}} \\
            & &&= \frac{(a + bi) \cdot (c + di)}{(c^2 + d^2)} \\
            & &&= \frac{(ac + bd) + (ad - bc)i}{c^2 + d^2} \\
            & &&= \frac{(ac + bd)}{c^2 + d^2} + \frac{(bc - ad)}{c^2 + d^2}i
        \end{alignat*}
    }
\end{minipage}
\begin{minipage}{0.4\linewidth}
    \noindent
    \parbox[t]{0.35\linewidth}
    {
        \begin{alignat*}{2}
            & z &&= \frac{1}{v} \\
            & &&= \frac{1}{v} \cdot \frac{\bar{v}}{\bar{v}} \\
            & &&= \frac{\bar{v}}{v \cdot \bar{v}} \\
            & &&= \frac{a + bi}{(a^2 + b^2)} \\
            & &&= \frac{a}{a^2 + b^2} - \frac{b}{a^2 + b^2}i
        \end{alignat*}
    }
\end{minipage}